separating interpolation into a function

code/theories/Interpolation.v
@@ -1,4 +1,5 @@
 From Stdlib Require Import Relations Arith Lia Bool List RelationClasses.
+From Equations Require Import Equations.
 From Interpolation Require Import Utils Syntax Languages Notations Reduction Typing Bidir.
 
 (** ** Primitives for context splitting *)
@@ -10,41 +11,50 @@ Section Splitting.
 
   Definition flip_side s := match s with | source => target | target => source end.
 
-  Inductive split : context -> context -> context -> Set :=
-    | split_emp : split ε ε ε
-    | split_s {Γ Γs Γt A} : split Γ Γs Γt -> split (Γ,,A) (Γs,,A) Γt
-    | split_t {Γ Γs Γt A} : split Γ Γs Γt -> split (Γ,,A) Γs (Γt,,A).
+  Inductive split : Set := 
+  | split_emp : split
+  | split_s : split -> split
+  | split_t : split -> split.
 
-  Fixpoint flip_split {Γ Γs Γt} (s : split Γ Γs Γt) : split Γ Γt Γs :=
+  Inductive splits : context -> context -> context -> split -> Prop :=
+    | splits_emp : splits ε ε ε split_emp
+    | splits_s {Γ Γs Γt A} {s} : splits Γ Γs Γt s -> splits (Γ,,A) (Γs,,A) Γt (split_s s)
+    | splits_t {Γ Γs Γt A} {s} : splits Γ Γs Γt s -> splits (Γ,,A) Γs (Γt,,A) (split_t s).
+
+  Fixpoint flip_split s : split :=
     match s with
     | split_emp => split_emp
     | split_s s => split_t (flip_split s)
     | split_t s => split_s (flip_split s)
     end.
 
-  Fixpoint sren_s {Γ Γs Γt} (s : split Γ Γs Γt) : ren :=
+  Fixpoint flip_splits {Γ Γs Γt} s : (splits Γ Γs Γt s) -> splits Γ Γt Γs (flip_split s).
+  Proof.
+    induction 1 ; cbn ; now constructor.
+  Qed.
+
+  Fixpoint sren_s (s : split) : ren :=
     match s with
     | split_emp => id
     | split_s s' => ⇑ (sren_s s')
     | split_t s' => (sren_s s') >> ↑
     end.
 
-  Fixpoint sren_t {Γ Γs Γt} (s : split Γ Γs Γt) : ren :=
+  Fixpoint sren_t (s : split) : ren :=
     match s with
     | split_emp => id
     | split_t s' => ⇑ (sren_t s')
     | split_s s' => (sren_t s') >> ↑
     end.
 
-  Lemma flip_split_inv {Γ Γs Γt} (s : split Γ Γs Γt) :
-    flip_split (flip_split s) = s.
+  Lemma flip_split_inv (s : split) : flip_split (flip_split s) = s.
   Proof.
     induction s ; cbn.
     1: easy.
     all: now rewrite IHs.
   Qed.
 
-  Lemma sren_s_flip {Γ Γs Γt} (s : split Γ Γs Γt) :
+  Lemma sren_s_flip (s : split) :
     sren_s (flip_split s) = sren_t s.
   Proof.
     induction s ; cbn.
@@ -52,7 +62,7 @@ Section Splitting.
     all: now rewrite IHs.
   Qed.
 
-  Lemma sren_t_split {Γ Γs Γt} (s : split Γ Γs Γt) :
+  Lemma sren_t_split (s : split) :
     sren_t (flip_split s) = sren_s s.
   Proof.
     rewrite <- (flip_split_inv s) at 2.
@@ -60,291 +70,751 @@ Section Splitting.
     reflexivity.
   Qed.
 
-  Lemma sren_s_ty {Γ Γs Γt} (s : split Γ Γs Γt) :
+  Lemma sren_s_ty {Γ Γs Γt} s :
+    splits Γ Γs Γt s ->
     Γ ⊢ (sren_s s) :: Γs.
   Proof.
-    induction s ; cbn.
+    induction 1 ; cbn.
     all: eauto with typing.
   Qed.
 
-  Lemma sren_t_ty {Γ Γs Γt} (s : split Γ Γs Γt) :
+  Lemma sren_t_ty {Γ Γs Γt} s :
+    splits Γ Γs Γt s ->
     Γ ⊢ (sren_t s) :: Γt.
   Proof.
+    intros.
     eapply ren_typing_ext.
-    2: eapply sren_s_ty.
-    rewrite sren_s_flip.
-    reflexivity.
+    2: now eapply sren_s_ty, flip_splits.
+    now rewrite sren_s_flip.
   Qed.
 
   Hint Resolve sren_s_ty sren_t_ty : typing.
 
-  Fixpoint find_side {Γ Γs Γt} (s : split Γ Γs Γt) (n : nat) : option side :=
+  Fixpoint find_side (s : split) (n : nat) : (option side*nat) :=
     match s, n with
-    | split_emp, _ => None
-    | split_s _, 0 => Some source
-    | split_t _, 0 => Some target
-    | split_s s', S n' | split_t s', S n' => find_side s' n'
+    | split_emp, _ => (None,0)
+    | split_s _, 0 => (Some source,0)
+    | split_t _, 0 => (Some target,0)
+    | split_s s', S n' => match (find_side s' n') with
+      | (None,_) => (None,0)
+      | (Some source,k) => (Some source,S k)
+      | (Some target,k) => (Some target,k)
+      end
+    | split_t s', S n' => match (find_side s' n') with
+      | (None,_) => (None,0)
+      | (Some source,k) => (Some source,k)
+      | (Some target,k) => (Some target,S k)
+      end
     end.
 
-  Lemma find_flip {Γ Γs Γt} (s : split Γ Γs Γt) (n : nat) :
-    find_side (flip_split s) n = option_map flip_side (find_side s n).
+  Lemma find_flip (s : split) (n : nat) :
+    find_side (flip_split s) n = prod_map (option_map flip_side) id (find_side s n).
   Proof.
     induction s in n |- * ; cbn ; try easy.
-    all: now destruct n ; cbn.
+    all: destruct n ; cbn ; try easy.
+    all: specialize (IHs n).
+    all: destruct (find_side (flip_split s) n) as [[[]|]]; cbn in * ; subst.
+    all: destruct (find_side _ _) as [[[]|]] ; cbn in * ; congruence.
   Qed.
 
-  Lemma in_context_find_none {Γ Γs Γt} (n : nat) (s : split Γ Γs Γt) T :
+  Lemma in_context_find_none {Γ Γs Γt} (n : nat) s T n' :
+    splits Γ Γs Γt s ->
     in_context n Γ T ->
-    find_side s n = None ->
+    find_side s n = (None,n') ->
     False.
   Proof.
-    induction s in n |- * ; [|destruct n | destruct n] ; cbn.
+    induction 1 in n, n' |- * ; [|destruct n | destruct n] ; cbn.
     - eauto with typing.
     - congruence.
-    - intros Hin ?%IHs.
-      1: easy.
-      exact Hin.
+    - intros Hin e.
+      destruct find_side as [[[]|]] eqn:? ; cbn in * ; solve [congruence|eauto].
     - congruence.
-    - intros Hin ?%IHs.
-      1: easy.
-      exact Hin.
+    - intros Hin e.
+      destruct find_side as [[[]|]] eqn:? ; cbn in * ; solve [congruence|eauto].
   Qed.
 
-  Lemma find_side_some_l {Γ Γs Γt} (n : nat) (s : split Γ Γs Γt) :
-    find_side s n = Some source ->
-    {n' & {T & in_context n' Γs T /\ n = sren_s s n'}}.
+  Lemma find_side_some_l {Γ Γs Γt} (n : nat) s n':
+    splits Γ Γs Γt s ->
+    find_side s n = (Some source,n') ->
+    exists T, in_context n' Γs T /\ n = sren_s s n'.
   Proof.
-    intros Hside.
-    induction s in n, Hside |- * ; [|destruct n | destruct n] ; cbn in *.
+    intros Hs Hside.
+    induction Hs in n, n', Hside |- * ; [|destruct n | destruct n] ; cbn in *.
     - congruence.
-    - eexists 0, _ ; split ; reflexivity.
-    - edestruct IHs as (n'&e&[]) ; tea.
+    - injection Hside ; subst.
+      eexists ; split ; reflexivity.
+    - destruct find_side as [[[]|]] eqn:e ; try solve [congruence].
+      injection Hside ; subst.
+      edestruct IHHs as (e'&[]) ; tea.
       subst.
-      eexists (S n'),_ ; split ; cbn ; tea ; reflexivity.
+      eexists ; split ; cbn ; tea ; reflexivity.
     - congruence.
-    - edestruct IHs as (n'&e&[]) ; tea.
+    - destruct find_side as [[[]|]] eqn:e ; try solve [congruence].
+      injection Hside ; subst.
+      edestruct IHHs as (e'&[]) ; tea.
       subst.
-      eexists n',_ ; split ; cbn ; tea ; reflexivity.
+      eexists ; split ; cbn ; tea ; reflexivity.
   Qed.
 
-  Lemma find_side_some_r {Γ Γs Γt} (n : nat) (s : split Γ Γs Γt) :
-    find_side s n = Some target ->
-    {n' & {T & in_context n' Γt T /\ n = sren_t s n'}}.
+  Lemma find_side_some_r {Γ Γs Γt} (n : nat) s n' :
+    splits Γ Γs Γt s ->
+    find_side s n = (Some target,n') ->
+    exists T, in_context n' Γt T /\ n = sren_t s n'.
   Proof.
-    intros e.
+    intros ? e.
     rewrite <- sren_s_flip.
-    apply find_side_some_l.
-    rewrite find_flip, e.
-    reflexivity.
+    eapply find_side_some_l.
+    1: now apply flip_splits.
+    now rewrite find_flip, e.
   Qed.
 
 End Splitting.
 
+Section Interpolant.
+  Context `{Lang}.
+
+  #[derive(eliminator=no)]Equations infer (Γ : context) (t : term) : type :=
+  infer Γ (tVar n)
+    with (nth_error Γ n) => {
+    | None => TUnit ;
+    | Some T => T
+    } ;
+  infer _ (tConst c) := const_type c ;
+  infer Γ (tApp f u)
+    with (infer Γ f) => {
+      | TFun _ B => B
+      | _ => TUnit
+    } ;
+  infer Γ (tProj b t)
+    with (infer Γ t) => {
+      | TProd A B => if b then A else B
+      | _ => TUnit
+    } ; 
+  infer _ _ => TUnit.
+
+  Lemma infer_infer Γ A t :
+  (Γ ⊢ t ▹ A) ->
+  infer Γ t = A.
+  Proof.
+    intros Hty.
+    pattern Γ, A, t.
+    revert Hty.
+    unshelve eapply bidir_ind.
+    1: intros ; exact True.
+    all: cbn ; try easy.
+    all: intros ; simp infer ; cbn.
+    - unfold in_context in *.
+      destruct nth_error ; cbn ; congruence.
+    - now rewrite H1 ; cbn.
+    - now rewrite H1 ; cbn.
+  Qed.
+
+  Let defaulti : side*type*term*term := (source,TUnit,tStar,tStar).
+
+  #[derive(eliminator=no)]Equations
+  _interpolate_infer (interp : forall (s : split) (c : const_split)
+      (Γ : context) (A : type) (t : term), type*term*term)
+    (s : split) (c : const_split) (Γ : context) (t : term) : side*type*term*term :=
+
+  _interpolate_infer _ s c Γ (tVar n)
+    with (find_side s n) => {
+      | (Some source,n') := (source,TUnit,tStar,(tVar (S n')))
+      | (Some target,n') := (target, TUnit,tStar,(tVar (S n')))
+      | (None, _) := defaulti
+    } ;
+  _interpolate_infer _ s csplit _ (tConst c)
+    with (const_cover csplit c) => {
+      | inl _ => (source,TUnit,tStar,(tConst c))
+      | inr _ => (target,TUnit,tStar,(tConst c))
+    } ;
+  _interpolate_infer interp s c Γ (tApp f u)
+    with (_interpolate_infer interp s c Γ f), (infer Γ f) => {
+    | (source,Mf,lf,rf), (TFun A _) :=
+        let '(Mu,lu,ru) := (interp (flip_split s) (flip_csplit c) Γ A u) in
+        (source,(TProd Mf Mu),(tPair lf lu),(tApp (rf[tip tFst]) (ru[(tip tSnd)])))
+    | (target,Mf,lf,rf), (TFun A _) :=
+        let '(Mu,lu,ru) := (interp s c Γ A u)
+        in (target,(TProd Mf Mu),(tPair lf lu),(tApp (rf[tip tFst]) (ru[(tip tSnd)])))
+    | _, _ := defaulti
+    } ;
+
+  _interpolate_infer interp s c Γ (tProj b t) :=
+    let '(o,M,l,r) := (_interpolate_infer interp s c Γ t) in
+    (o,M,l,(tProj b r)) ;
+
+  _interpolate_infer _ _ _ _ _ := defaulti.
+
+  Let default := (TUnit,tStar,tStar).
+
+  #[derive(eliminator=no)]Equations
+  interpolate (s : split) (c : const_split) (Γ : context) (A : type) (t : term)
+    : type*term*term :=
+  
+  interpolate s c Γ _ tStar :=
+    (TUnit,tStar,tStar) ;
+
+  interpolate s c Γ (TFun A B) (tLam t) =>
+    let '(M,l,r) := (interpolate (split_t s) c (Γ,,A) B t)
+    in (M,l,tLam (r⟨swap_var⟩)) ;
+  interpolate _ _ _ _ (tLam _) =>
+    default ;
+
+  interpolate s c Γ (TProd A B) (tPair t t') :=
+    let '(M,l,r) := (interpolate s c Γ A t)
+    in let '(M',l',r') := (interpolate s c Γ B t')
+    in ((TProd M M'),(tPair l l'),(tPair (r[tip tFst]) (r'[tip tSnd]))) ;
+  interpolate _ _ _ _ (tPair _ _) =>
+    default ;
+
+  interpolate s c Γ (TSum A B) (tIn b t) :=
+    let '(M,l,r) := (interpolate s c Γ (if b then A else B) t)
+    in (M, l, (tIn b r)) ;
+  interpolate _ _ _ _ (tIn b t) :=
+    default ;
+
+  interpolate s c Γ _ (tAbort t)
+    with (_interpolate_infer interpolate s c Γ t) => {
+    | (source,M,l,r) :=
+        ((TFun M TEmp),(tLam r),(tAbort (tApp (tVar 0) l⟨↑⟩)))
+    | (target,M,l,r) := (M, l, (tAbort r))
+    } ;
+
+  interpolate s c Γ C (tIf t bl br)
+    with (_interpolate_infer interpolate s c Γ t), (infer Γ t) => {
+
+    | (source,M,l,r), TSum A B :=
+      let '(Ml,ll,rl) := interpolate (split_s s) c (Γ,,A) C bl
+      in let '(Mr,lr,rr) := interpolate (split_s s) c (Γ,,B) C br
+      in ((TFun M (TSum Ml Mr)),
+          (tLam (tIf r (tLeft ll⟨↑⟩⟨swap_var⟩) (tRight lr⟨↑⟩⟨swap_var⟩))),
+          (tIf (tApp (tVar 0) l⟨↑⟩) rl⟨↑⟩⟨swap_var⟩ rr⟨↑⟩⟨swap_var⟩)) ;
+
+    | (target,M,l,r), TSum A B :=
+      let '(Ml,ll,rl) := interpolate (split_t s) c (Γ,,A) C bl
+      in let '(Mr,lr,rr) := interpolate (split_t s) c (Γ,,B) C br
+      in ((TProd M (TProd Ml Mr)),
+          (tPair l (tPair ll lr)),
+          ((tIf r[tip tFst]
+            rl[(tip (fun x => (tFst (tSnd x))))]⟨swap_var⟩
+            rr[(tip (fun x => tSnd (tSnd x)))]⟨swap_var⟩)))
+
+    | _, _ => default ;
+    } ;
+
+  interpolate s c Γ A i
+    with (_interpolate_infer interpolate s c Γ i) => {
+    | (source,M,l,r) :=
+        ((TFun M (infer Γ i)), (tLam r), (tApp (tVar 0) l⟨↑⟩))
+    | (target,M,l,r) := (M, l, r)
+    }.
+
+End Interpolant.
+
+Notation interpolate_infer := (_interpolate_infer interpolate).
+
+Lemma interpolate_infer_eq `{Lang} Γ A i s c :
+  (Γ ⊢ i ▹ A) ->
+  interpolate s c Γ A i =
+    (match (interpolate_infer s c Γ i) with 
+      | (source,M,l,r) =>
+        ((TFun M (infer Γ i)), (tLam r), (tApp (tVar 0) l⟨↑⟩))
+      | (target,M,l,r) => (M, l, r)
+    end).
+Proof.
+  intros Hty.
+  inversion Hty ; subst ; cbn.
+  - destruct _interpolate_infer_clause_1 as ((([]&?)&?)&?) ; cbn ; reflexivity.
+  - destruct _interpolate_infer_clause_2 as ((([]&?)&?)&?) ; cbn ; reflexivity.
+  - destruct _interpolate_infer_clause_3 as ((([]&?)&?)&?) ; cbn ; reflexivity.
+  - destruct interpolate_infer as ((([]&?)&?)&?) ; cbn ; reflexivity.
+Qed.
+  
 Section Interpolation.
   Context `{Lang}.
 
-  (** With the splitting of the context given by Γs and Γt and the type A,
-    I is a valid interpolating type. *)
-  Definition interpolate_ty Γs Γt A M (c : const_split): Prop :=
-    forall p, atoms_ty p M ⊆ 
+    Let Pcheck_lang_ty Γ T t := forall Γs Γt (s : split) (c : const_split),
+    splits Γ Γs Γt s ->
+    let '(M,l,r) := interpolate s c Γ T t in
+    forall p,
+    atoms_ty p M ⊆ 
       (atoms_ctx p Γs ∪ atoms_const p c.(pconst_l)) ∩
-      (atoms_ctx (negp p) Γt ∪ (atoms_const (negp p) c.(pconst_r)) ∪ atoms_ty p A).
+        (atoms_ctx (negp p) Γt ∪ (atoms_const (negp p) c.(pconst_r)) ∪ atoms_ty p T).
 
-  Definition interpolate_tm {Γ Γs Γt} (s : split Γ Γs Γt) (c : const_split) M A t l r :=
-    (Γs ⊢ l :: M) /\ (atoms_tm l ⊆ c.(pconst_l)) /\
-    (Γt ,, M ⊢ r :: A) /\ (atoms_tm r ⊆ c.(pconst_r)) /\
-    r⟨⇑ (sren_t s)⟩[l⟨sren_s s⟩..] ⤳* t.
-
-  Let Pcheck Γ T t := forall Γs Γt (s : split Γ Γs Γt) (c : const_split),
-    exists M l r,
-      interpolate_ty Γs Γt T M c /\ interpolate_tm s c M T t l r.
-
-  Let Pinf Γ T t := forall Γs Γt (s : split Γ Γs Γt) (c : const_split),
-    (
-      (forall p, atoms_ty p T ⊆ atoms_ctx p Γt ∪ atoms_const p c.(pconst_r)) /\
-      (exists M l r, 
-        (forall p, atoms_ty p M ⊆ (atoms_ctx p Γs ∪ atoms_const p c.(pconst_l))
-                                  ∩ (atoms_ctx (negp p) Γt ∪ atoms_const (negp p) c.(pconst_r)))
-        /\ interpolate_tm s c M T t l r)
-    ) \/ (
-      (forall p, atoms_ty p T ⊆ atoms_ctx p Γs ∪ atoms_const p c.(pconst_l)) /\
-      (exists M l r, 
-        (forall p, atoms_ty p M ⊆ (atoms_ctx (negp p) Γs ∪ atoms_const (negp p) c.(pconst_l))
-                                  ∩ (atoms_ctx p Γt ∪ atoms_const p c.(pconst_r)))
-        /\ interpolate_tm (flip_split s) (flip_csplit c) M T t l r)
-    ).
-
-  Ltac pre_crush_incl :=
-    unfold interpolate_ty in * ;
-    intros ;
-    repeat match goal with
-      | b : polarity |- _ => destruct b
-      | H : forall b : polarity, _ |- _ => pose proof (H pos) ; pose proof (H neg) ; cbn in * ; clear H
+  Let Pinf_lang_ty Γ (T : type) t := forall Γs Γt (s : split) (c : const_split),
+    splits Γ Γs Γt s ->
+    let '(si,M,l,r) := interpolate_infer s c Γ t in
+    match si with
+    | target => 
+        (forall p, atoms_ty p T ⊆ atoms_ctx p Γt ∪ atoms_const p c.(pconst_r))
+        /\ (forall p, atoms_ty p M ⊆ (atoms_ctx p Γs ∪ atoms_const p c.(pconst_l))
+                                      ∩ (atoms_ctx (negp p) Γt ∪ atoms_const (negp p) c.(pconst_r)))
+    | source =>
+        (forall p, atoms_ty p T ⊆ atoms_ctx p Γs ∪ atoms_const p c.(pconst_l))
+        /\ (forall p, atoms_ty p M ⊆ (atoms_ctx (negp p) Γs ∪ atoms_const (negp p) c.(pconst_l))
+                                      ∩ (atoms_ctx p Γt ∪ atoms_const p c.(pconst_r)))
     end.
 
-  Ltac crush_incl := pre_crush_incl ; set_solver.
-
-  Theorem interpolation_ind : bidir_concl Pcheck Pinf.
+  Lemma polarity_reverse (P : polarity -> polarity -> Prop) :
+    (forall p, P (negp p) p) ->
+    (forall p, P p (negp p)).
   Proof.
-    apply bidir_ind ; subst Pcheck Pinf.
+    intros HP.
+    destruct p ; cbn.
+    - apply (HP neg).
+    - apply (HP pos).
+  Qed.
+
+  Theorem interpolation_lang_ty : bidir_concl Pcheck_lang_ty Pinf_lang_ty.
+  Proof.
+    subst Pcheck_lang_ty Pinf_lang_ty ; clear.
+    apply bidir_ind ; cbn in *.
 
     - (* case tStar *)
-      intros Γ Γs Γt s.
-      exists TUnit, tStar, tStar.
-      split.
-      1: solve [crush_incl].
-      red.
-      prod_splitter.
-      1,3: now auto with typing.
-      1,2: solve [crush_incl].
+      intros.
+      set_solver.
+
+    - (* case tLam *)
+      intros * _ IH * Hs ; cbn.
+      specialize (IH _ _ _ c (splits_t Hs)).
+      destruct interpolate as ((?&?)&?) ; cbn.
+      set_solver.
+    
+    - (* case tPair *)
+      intros * _ IHA _ IHB * Hs.
+      specialize (IHA _ _ _ c Hs).
+      specialize (IHB _ _ _ c Hs).
+      destruct interpolate as ((?&?)&?) ; cbn.
+      destruct interpolate as ((?&?)&?) ; cbn.
+      all: set_solver.
+    
+    - (* case tLeft *)
+      intros * _ IH * Hs.
+      specialize (IH _ _ _ c Hs).
+      (destruct interpolate as ((?&?)&?) ; cbn).
+      set_solver.
+    
+    - (* case tRight *)
+      intros * _ IH * Hs.
+      specialize (IH _ _ _ c Hs).
+      (destruct interpolate as ((?&?)&?) ; cbn).
+      set_solver.
+    
+    - (* case tAbort *)
+      intros * _ IH * Hs.
+      specialize (IH _ _ _ c Hs).
+      destruct interpolate_infer as ((([]&?)&?)&?) ; cbn in *.
+      + intros.
+        pattern p, (negp p).
+        apply polarity_reverse.
+        set_solver.
+      + set_solver. 
+
+    - (* case tIf *)
+      intros * ? IHs _ IHl _ IHr * Hs.
+      specialize (IHs _ _ _ c Hs) ; cbn in *.
+      destruct interpolate_infer as ((([]&Ms)&rs)&ls) ; cbn in *.
+      all: destruct IHs as [IHT IHs].
+      all: red ; erewrite infer_infer ; tea ; cbn.
+      + specialize (IHl _ _ _ c (splits_s Hs)) ; cbn in *.
+        destruct interpolate as ((Ml&ll)&rl) ; cbn in *.
+        specialize (IHr _ _ _ c (splits_s Hs)) ; cbn in *.
+        destruct interpolate as ((Mr&lr)&rr) ; cbn in *.
+        intros.
+        repeat apply union_least.
+        * clear -IHs.
+          pattern p, (negp p).
+          apply polarity_reverse.
+          intros.
+          set_solver.
+        * clear -IHT IHl.
+          set_solver.
+        * clear -IHT IHr.
+          set_solver.
+
+      + specialize (IHl _ _ _ c (splits_t Hs)) ; cbn in *.
+        destruct interpolate as ((Ml&ll)&rl) ; cbn in *.
+        specialize (IHr _ _ _ c (splits_t Hs)) ; cbn in *.
+        destruct interpolate as ((Mr&lr)&rr) ; cbn in *.
+        intros.
+        repeat apply union_least.
+        * clear -IHs.
+          set_solver.
+        * clear -IHT IHl.
+          set_solver.
+        * clear -IHT IHr.
+          set_solver.
+
+    - (* case demote *)
+      intros * ? IH -> * Hs.
+      specialize (IH _ _ _ c Hs).
+      rewrite interpolate_infer_eq ; tea.
+      erewrite infer_infer ; tea ; cbn.
+      destruct interpolate_infer as ((([]&?)&?)&?) ; cbn in *.
+      all: destruct IH.
+      + intros.
+        apply union_least.
+        * pattern p, (negp p).
+          apply polarity_reverse.
+          set_solver.
+        * set_solver.
+      + set_solver.
+
+    - (* case tVar *)
+      intros * Hin * Hs.
+      destruct (find_side s n) as ([[]|]&?) eqn:e.
+      + eapply find_side_some_l in e as (A&[? ->]) ; tea ; cbn.
+        eapply in_context_inj in Hin.
+        2:now eapply sren_s_ty.
+        subst.
+        split.
+        1: intros ; rewrite atoms_in ; tea ; set_solver.
+        set_solver.
+      + eapply find_side_some_r in e as (A&[? ->]) ; tea ; cbn.
+        eapply in_context_inj in Hin.
+        2:now eapply sren_t_ty.
+        subst.
+        split.
+        1: intros ; rewrite atoms_in ; tea ; set_solver.
+        set_solver.
+      + exfalso ; now eauto using in_context_find_none. 
+
+    - (* case tConst *)
+      intros * Hs.
+      destruct const_cover ; cbn.
+      all: set_solver.
+
+    - (* case tApp *)
+      intros * ? IHf _ IHu * Hs.
+      specialize (IHf _ _ _ c Hs).
+      destruct interpolate_infer as ((([]&?)&?)&?) ; cbn in *.
+      all: red ; erewrite infer_infer ; tea ; cbn.
+      1: specialize (IHu _ _ _ (flip_csplit c) (flip_splits _ Hs)) ; cbn in *.
+      2: specialize (IHu _ _ _ c Hs) ; cbn in *.
+      all: destruct interpolate as ((?&?)&?) ; cbn.
+      all: split ; [set_solver|].
+      all: intros p.
+      all: destruct IHf as (IHty&?).
+      all: specialize (IHty (negp p)).
+      all: rewrite negp_inv in IHty.
+      all: set_solver.
+
+    - (* case tProj *)
+      intros * _ IH * Hs.
+      specialize (IH _ _ _ c Hs).
+      destruct interpolate_infer as ((([]&?)&?)&?) ; cbn in *.
+      all: destruct b.
+      all: set_solver.
+  Qed.
+
+    Let Pcheck_ty Γ T t := forall Γs Γt (s : split) (c : const_split),
+    splits Γ Γs Γt s ->
+    let '(M,l,r) := interpolate s c Γ T t in
+    (Γs ⊢ l :: M) /\ (Γt ,, M ⊢ r :: T).
+
+  Let Pinf_ty Γ (T : type) t := forall Γs Γt (s : split) (c : const_split),
+    splits Γ Γs Γt s ->
+    let '(si,M,l,r) := interpolate_infer s c Γ t in
+    match si with
+    | target => (Γs ⊢ l :: M) /\ (Γt ,, M ⊢ r :: T)
+    | source => (Γt ⊢ l :: M) /\ (Γs ,, M ⊢ r :: T)
+    end.
+
+  Theorem interpolation_ty : bidir_concl Pcheck_ty Pinf_ty.
+  Proof.
+    subst Pcheck_ty Pinf_ty ; clear.
+    apply bidir_ind ; cbn in *.
+
+    - (* case tStar *)
+      intros.
+      eauto with typing.
+
+    - (* case tLam *)
+      intros * _ IH * Hs ; cbn.
+      specialize (IH _ _ _ c (splits_t Hs)).
+      destruct interpolate as ((?&?)&?) ; cbn.
+      eauto with typing.
+    
+    - (* case tPair *)
+      intros * _ IHA _ IHB * Hs.
+      specialize (IHA _ _ _ c Hs).
+      specialize (IHB _ _ _ c Hs).
+      destruct interpolate as ((?&?)&?) ; cbn.
+      destruct interpolate as ((?&?)&?) ; cbn.
+      eauto 20 with typing.
+    
+    - (* case tLeft *)
+      intros * _ IH * Hs.
+      specialize (IH _ _ _ c Hs).
+      (destruct interpolate as ((?&?)&?) ; cbn).
+      eauto 20 with typing.
+    
+    - (* case tRight *)
+      intros * _ IH * Hs.
+      specialize (IH _ _ _ c Hs).
+      (destruct interpolate as ((?&?)&?) ; cbn).
+      eauto 20 with typing.
+    
+    - (* case tAbort *)
+      intros * _ IH * Hs.
+      specialize (IH _ _ _ c Hs).
+      destruct interpolate_infer as ((([]&M)&l)&r) ; cbn in *.
+      all: eauto 10 with typing.
+
+    - (* case tIf *)
+      intros * ? IHs _ IHl _ IHr * Hs.
+      specialize (IHs _ _ _ c Hs).
+      destruct interpolate_infer as ((([]&?)&l)&r) ; cbn in *.
+      1: specialize (IHl _ _ _ c (splits_s Hs)) ; cbn in *.
+      2: specialize (IHl _ _ _ c (splits_t Hs)) ; cbn in *.
+      1: specialize (IHr _ _ _ c (splits_s Hs)) ; cbn in *.
+      2: specialize (IHr _ _ _ c (splits_t Hs)) ; cbn in *.
+      all: red ; erewrite infer_infer ; tea ; cbn.
+      all: do 2 (destruct interpolate as ((?&?)&?) ; cbn in *).
+      + split ; eauto 20 with typing.
+      + split.
+        all: eauto 30 with typing.
+
+    - (* case demote *)
+      intros * ? IH -> * Hs.
+      specialize (IH _ _ _ c Hs).
+      rewrite interpolate_infer_eq ; tea.
+      destruct interpolate_infer as ((([]&?)&?)&?) ; cbn in *.
+      1: erewrite infer_infer ; tea.
+      all: split ; eauto 10 with typing.
+
+    - (* case tVar *)
+      intros * Hin * Hs.
+      destruct (find_side s n) as ([[]|]&?) eqn:e.
+      + eapply find_side_some_l in e as (A&[? ->]) ; tea ; cbn.
+        eapply in_context_inj in Hin.
+        2:now eapply sren_s_ty.
+        subst.
+        eauto with typing.
+      + eapply find_side_some_r in e as (A&[? ->]) ; tea ; cbn.
+        eapply in_context_inj in Hin.
+        2:now eapply sren_t_ty.
+        subst.
+        eauto with typing.
+      + exfalso ; now eauto using in_context_find_none.
+
+    - (* case tConst *)
+      intros * Hs.
+      destruct const_cover ; cbn.
+      all: eauto with typing.
+
+    - (* case tApp *)
+      intros * ? IHf _ IHu * Hs.
+      specialize (IHf _ _ _ c Hs).
+      destruct interpolate_infer as ((([]&?)&?)&?) ; cbn in *.
+      all: red ; erewrite infer_infer ; tea ; cbn.
+      + specialize (IHu _ _ _ (flip_csplit c) (flip_splits _ Hs)) ; cbn in *.
+        destruct interpolate as ((?&?)&?) ; cbn.
+        eauto 20 with typing.
+
+      + specialize (IHu _ _ _ c Hs) ; cbn in *.
+        destruct interpolate as ((?&?)&?) ; cbn.
+        eauto 20 with typing.
+
+    - (* case tProj *)
+      intros * _ IH * Hs.
+      specialize (IH _ _ _ c Hs).
+      destruct interpolate_infer as ((([]&?)&?)&?) ; cbn in *.
+      all: destruct b ; eauto 20 with typing.
+  Qed.
+
+  Let Pcheck_lang_tm Γ T t := forall Γs Γt (s : split) (c : const_split),
+    splits Γ Γs Γt s ->
+    let '(M,l,r) := interpolate s c Γ T t in
+    (atoms_tm l ⊆ c.(pconst_l)) /\ (atoms_tm r ⊆ c.(pconst_r)).
+
+  Let Pinf_lang_tm Γ (T : type) t := forall Γs Γt (s : split) (c : const_split),
+    splits Γ Γs Γt s ->
+    let '(si,M,l,r) := interpolate_infer s c Γ t in
+    match si with
+    | source => (atoms_tm l ⊆ (flip_csplit c).(pconst_l)) /\ (atoms_tm r ⊆ (flip_csplit c).(pconst_r)) 
+    | target => (atoms_tm l ⊆ c.(pconst_l)) /\ (atoms_tm r ⊆ c.(pconst_r))
+    end.
+
+  Theorem interpolation_lang_tm : bidir_concl Pcheck_lang_tm Pinf_lang_tm.
+  Proof.
+    subst Pcheck_lang_tm Pinf_lang_tm ; clear.
+    apply bidir_ind ; cbn in *.
+
+    - (* case tStar *)
+      intros.
+      set_solver.
+
+    - (* case tLam *)
+      intros * _ IH * Hs ; cbn.
+      specialize (IH _ _ _ c (splits_t Hs)).
+      destruct interpolate as ((?&?)&?) ; cbn.
+      rewrite atoms_ren.
+      set_solver.
+    
+    - (* case tPair *)
+      intros * _ IHA _ IHB * Hs.
+      specialize (IHA _ _ _ c Hs).
+      specialize (IHB _ _ _ c Hs).
+      destruct interpolate as ((?&?)&?) ; cbn.
+      destruct interpolate as ((?&?)&?) ; cbn.
+      rewrite !atoms_subst_tip_eq ; cbn.
+      all: set_solver.
+    
+    - (* case tLeft *)
+      intros * ? * _ IH * Hs.
+      specialize (IH _ _ _ c Hs).
+      (destruct interpolate as ((?&?)&?) ; cbn).
+      set_solver.
+    
+    - (* case tRight *)
+      intros * ? * _ IH * Hs.
+      specialize (IH _ _ _ c Hs).
+      (destruct interpolate as ((?&?)&?) ; cbn).
+      set_solver.
+    
+    - (* case tAbort *)
+      intros * _ IH * Hs.
+      specialize (IH _ _ _ c Hs).
+      destruct interpolate_infer as ((([]&?)&?)&?) ; cbn in *.
+      1: rewrite atoms_ren.
+      all: set_solver.
+
+    - (* case tIf *)
+      intros * ? IHs _ IHl _ IHr * Hs.
+      specialize (IHs _ _ _ c Hs).
+      destruct interpolate_infer as ((([]&?)&?)&?) ; cbn in *.
+      1: specialize (IHl _ _ _ c (splits_s Hs)) ; cbn in *.
+      2: specialize (IHl _ _ _ c (splits_t Hs)) ; cbn in *.
+      1: specialize (IHr _ _ _ c (splits_s Hs)) ; cbn in *.
+      2: specialize (IHr _ _ _ c (splits_t Hs)) ; cbn in *.
+      all: red ; erewrite infer_infer ; tea ; cbn.
+      all: do 2 (destruct interpolate as ((?&?)&?) ; cbn in *).
+      all: rewrite ?atoms_ren, ?atoms_subst_tip_eq ; cbn.
+      all: set_solver.
+
+    - (* case demote *)
+      intros * ? IH -> * Hs.
+      specialize (IH _ _ _ c Hs).
+      rewrite interpolate_infer_eq ; tea.
+      destruct interpolate_infer as ((([]&?)&?)&?) ; cbn in *.
+      all: rewrite ?atoms_ren.
+      all: set_solver.
+
+    - (* case tVar *)
+      intros * Hin * Hs.
+      destruct (find_side s n) as ([[]|]&?) eqn:e.
+      3: exfalso ; now eauto using in_context_find_none.
+      + eapply find_side_some_l in e as (A&[? ->]) ; tea ; cbn.
+        set_solver.
+      + eapply find_side_some_r in e as (A&[? ->]) ; tea ; cbn.
+        set_solver.
+
+    - (* case tConst *)
+      intros * Hs.
+      destruct const_cover ; cbn.
+      all: set_solver.
+
+    - (* case tApp *)
+      intros * ? IHf _ IHu * Hs.
+      specialize (IHf _ _ _ c Hs).
+      destruct interpolate_infer as ((([]&?)&?)&?) ; cbn in *.
+      all: red ; erewrite infer_infer ; tea ; cbn.
+      + specialize (IHu _ _ _ (flip_csplit c) (flip_splits _ Hs)) ; cbn in *.
+        destruct interpolate as ((?&?)&?) ; cbn.
+        rewrite !atoms_subst_tip_eq ; cbn in *.
+        all: set_solver.
+
+      + specialize (IHu _ _ _ c Hs) ; cbn in *.
+        destruct interpolate as ((?&?)&?) ; cbn.
+        rewrite !atoms_subst_tip_eq ; cbn in *.
+        all: set_solver.
+
+    - (* case tProj *)
+      intros * _ IH * Hs.
+      specialize (IH _ _ _ c Hs).
+      destruct interpolate_infer as ((([]&?)&?)&?) ; cbn in *.
+      all: set_solver.
+  Qed.
+
+
+  Let Pcheck_red Γ T t := forall Γs Γt (s : split) (c : const_split),
+    splits Γ Γs Γt s ->
+    let '(M,l,r) := interpolate s c Γ T t in
+    r⟨⇑ (sren_t s)⟩[l⟨sren_s s⟩..] ⤳* t.
+
+  Let Pinf_red Γ (T : type) t := forall Γs Γt (s : split) (c : const_split),
+    splits Γ Γs Γt s ->
+    let '(si,M,l,r) := interpolate_infer s c Γ t in
+    match si with
+    | source => r⟨⇑ (sren_s s)⟩[l⟨sren_t s⟩..] ⤳* t
+    | target => r⟨⇑ (sren_t s)⟩[l⟨sren_s s⟩..] ⤳* t
+    end.
+
+  Theorem interpolation_red : bidir_concl Pcheck_red Pinf_red.
+  Proof.
+    subst Pcheck_red Pinf_red ; clear.
+    apply bidir_ind ; cbn in *.
+
+    - (* case tStar *)
+      intros.
       reflexivity.
 
     - (* case tLam *)
-      intros Γ A B t _ IH Γs Γt s c.
-      destruct (IH Γs (Γt,,A) (split_t s) c) as (M&l&r&HM&Ht).
-      exists M, l, (tLam (r⟨swap_var⟩)).
-      split.
-      1: clear -HM ; solve [crush_incl].
+      intros * _ IH * Hs ; cbn.
+      specialize (IH _ _ _ c (splits_t Hs)).
+      destruct interpolate as ((?&?)&?) ; cbn.
       
-      unfold interpolate_tm in * ; cbn in *.
-      destruct Ht as (?&?&?&?&e).
-      prod_splitter.
-      1,3: now eauto with typing.
-      1: solve [crush_incl].
-      1: rewrite atoms_ren ; solve [crush_incl].
-
       refold.
-      now rewrite swap_up2, swap_up1, renRen_term, e.
+      now rewrite swap_up2, swap_up1, renRen_term, IH.
     
     - (* case tPair *)
-      intros Γ A B t t' _ IHA _ IHB Γs Γt s c.
-      destruct (IHA Γs Γt s c) as (M & l & r & HM & (?&?&?&?&et)).
-      destruct (IHB Γs Γt s c) as (M' & l' & r' & HM' & (?&?&?&?&et')).
-      exists (TProd M M'), (tPair l l'),
-        (tPair (r[tip tFst]) (r'[tip tSnd])).
-      split.
-      1: clear -HM HM' ; solve [crush_incl].
-      
-      unfold interpolate_tm in * ; cbn in *.
-      prod_splitter.
-      1,3: now eauto 20 with typing.
-      1: solve [crush_incl].
-      + erewrite union_mono.
-        2-3: rewrite atoms_tm_subst, atoms_subst_tip ; cbn ; reflexivity.
-        set_solver.
-      
-      + now rewrite !tip_up_ren, !tip_subst, ST_Fst, ST_Snd, et, et'.
+      intros * _ IHA _ IHB * Hs.
+      specialize (IHA _ _ _ c Hs).
+      specialize (IHB _ _ _ c Hs).
+      destruct interpolate as ((?&?)&?) ; cbn.
+      destruct interpolate as ((?&?)&?) ; cbn.
+
+      now rewrite !tip_up_ren, !tip_subst, ST_Fst, ST_Snd, IHA, IHB.
     
-      - (* case tLeft *)
-      intros * _ IH ?? s c.
-      destruct (IH _ _ s c) as (M & l & r & HM & Ht).
-      exists M, l, (tLeft r).
-      split.
-      1: clear -HM ; solve [crush_incl].
-      
-      unfold interpolate_tm in * ; cbn in *.
-      destruct Ht as (?&?&?&?&e).
-      prod_splitter.
-      1,3: eauto with typing.
-      1-2: solve [crush_incl].
-      now rewrite e.
+    - (* case tLeft *)
+      intros * ? * _ IH * Hs.
+      specialize (IH _ _ _ c Hs).
+      (destruct interpolate as ((?&?)&?) ; cbn).
+      now rewrite IH.
     
     - (* case tRight *)
-      intros * _ IH ?? s c.
-      destruct (IH _ _ s c) as (M & l & r & HM & Ht).
-      exists M, l, (tRight r).
-      split.
-      1: clear -HM ; solve [crush_incl].
-
-      unfold interpolate_tm in * ; cbn in *.
-      destruct Ht as (?&?&?&?&e).
-      prod_splitter.
-      1,3: eauto with typing.
-      1-2: solve [crush_incl].
-      now rewrite e.
+      intros * ? * _ IH * Hs.
+      specialize (IH _ _ _ c Hs).
+      (destruct interpolate as ((?&?)&?) ; cbn).
+      now rewrite IH.
     
-      - (* case tAbort *)
-      intros * _ IH ?? s c.
-      destruct (IH _ _ s c) as [[_ (M&l&r&[HM (?&?&?&?&e)])]|[_ (M&l&r&[HM (?&?&?&?&e)])]] ; tea.
-
-      + exists M, l, (tAbort r).
-        split.
-        1: clear -HM ; solve [crush_incl].
-
-        unfold interpolate_tm in * ; cbn in *.
-        prod_splitter.
-        1,3: eauto with typing.
-        1-2: solve [crush_incl].
-        now rewrite e.
-
-      + exists (TFun M TEmp), (tLam r), (tAbort (tApp (tVar 0) l⟨↑⟩)).
-        split.
-        1: clear -HM ; solve [crush_incl].
-
-        unfold interpolate_tm in *.
-        prod_splitter.
-        1,3: eauto 20 with typing.
-        1: cbn in * ; solve [crush_incl].
-        1: cbn in * ; rewrite atoms_ren ; solve [crush_incl].
-
-        cbn ; refold.
-        rewrite ST_Beta_Fun.
-        rewrite sren_s_flip, sren_t_split in e.
-        apply R_Abort_cong.
-        etransitivity ; [|eassumption].
-        apply ereflexivity.
-        substify.
-        now asimpl.
+    - (* case tAbort *)
+      intros * _ IH * Hs.
+      specialize (IH _ _ _ c Hs).
+      destruct interpolate_infer as ((([]&M)&l)&r) ; cbn in *.
+      
+      2: now rewrite IH.
+      refold.
+      rewrite ST_Beta_Fun.
+      apply R_Abort_cong.
+      etransitivity ; [|eassumption].
+      apply ereflexivity.
+      substify.
+      now asimpl.
 
     - (* case tIf *)
-      intros Γ A B T s bl br ? IHs ? IHl ? IHr ?? sp c.
-      destruct (IHs _ _ sp c) as [[HMsum (M&l&r&[HMs (?&?&?&?&es)])]|[HMsum (M&l&r&[HMs (?&?&?&?&es)])]] ; tea.
-
-      + destruct (IHl _ _ (split_t sp) c) as (Ml & ll & rl & HMl & (?&?&?&?&etl)).
-        destruct (IHr _ _ (split_t sp) c) as (Mr & lr & rr & HMr & (?&?&?&?&etr)).
-        exists (TProd M (TProd Ml Mr)), (tPair l (tPair ll lr)),
-          ((tIf r[tip tFst]
-            rl[(tip (fun x => (tFst (tSnd x))))]⟨swap_var⟩
-            rr[(tip (fun x => tSnd (tSnd x)))]⟨swap_var⟩)).
-        split.
-        1: clear -HMsum HMs HMl HMr ; solve [crush_incl].
-
-        unfold interpolate_tm in *.
-        prod_splitter.
-        1,3: eauto 20 with typing.
-        1: solve [crush_incl].
-        * cbn.
-          etransitivity.
-          1: repeat apply union_mono ; rewrite ?atoms_ren, atoms_tm_subst, atoms_subst_tip ; cbn ; reflexivity.
-          set_solver.
-
-        * cbn ; refold.
-          rewrite !swap_up2, !swap_up1, !tip_up_ren, !tip_subst ; cbn ; try easy.
-          now rewrite !ST_Snd, !ST_Fst, renRen_term, renRen_term, etl, etr, es.
-
-      + rewrite sren_s_flip, sren_t_split in es.
-        destruct (IHl _ _ (split_s sp) c) as (Ml & ll & rl & HMl & (?&?&?&?&etl)).
-        destruct (IHr _ _ (split_s sp) c) as (Mr & lr & rr & HMr & (?&?&?&?&etr)).
-        exists (TFun M (TSum Ml Mr)),
-          (tLam (tIf r (tLeft ll⟨↑⟩⟨swap_var⟩) (tRight lr⟨↑⟩⟨swap_var⟩))),
-          (tIf (tApp (tVar 0) l⟨↑⟩) rl⟨↑⟩⟨swap_var⟩ rr⟨↑⟩⟨swap_var⟩).
-        split.
-        1: clear -HMsum HMs HMl HMr ; solve [crush_incl].
-
-      unfold interpolate_tm in *.
-      prod_splitter.
-      1,3: now eauto 20 with typing.
-      * cbn.
-        etransitivity.
-        1: repeat apply union_mono ; rewrite ?atoms_ren ; reflexivity.
-        set_solver.
-      * cbn.
-        etransitivity.
-        1: repeat apply union_mono ; rewrite ?atoms_ren ; reflexivity.
-        set_solver.
+      intros * ? IHs _ IHl _ IHr * Hs.
+      specialize (IHs _ _ _ c Hs).
+      destruct interpolate_infer as ((([]&?)&l)&r) ; cbn in *.
+      1: specialize (IHl _ _ _ c (splits_s Hs)) ; cbn in *.
+      2: specialize (IHl _ _ _ c (splits_t Hs)) ; cbn in *.
+      1: specialize (IHr _ _ _ c (splits_s Hs)) ; cbn in *.
+      2: specialize (IHr _ _ _ c (splits_t Hs)) ; cbn in *.
+      all: red ; erewrite infer_infer ; tea ; cbn.
+      all: do 2 (destruct interpolate as ((?&?)&?) ; cbn in *).
       
-      * cbn ; refold.
-        clear -es etl etr.
+      all: refold.
+      + cbn ; refold.
         rewrite !swap_up2, !swap_up1, !ST_Beta_Fun.
         cbn ; refold.
         rewrite ST_If_If, !ST_Left, !ST_Right, !swap_up2, !swap_up1 ; refold.
@@ -365,182 +835,58 @@ Section Interpolation.
            intros [|] ; cbn ; [|easy].
            now substify ; asimpl.
 
+      + rewrite !swap_up2, !swap_up1, !tip_up_ren, !tip_subst ; cbn ; try easy.
+        now rewrite !ST_Snd, !ST_Fst, renRen_term, renRen_term, IHs, IHl, IHr. 
+
     - (* case demote *)
-      intros * _ IH -> ?? s c.
-      destruct (IH _ _ s c) as [[? (M&l&r&[HM ?])]|[Hat (M&l&r&[HM (?&?&?&?&erl)])]] ; tea.
+      intros * ? IH -> * Hs.
+      specialize (IH _ _ _ c Hs).
+      rewrite interpolate_infer_eq ; tea.
+      destruct interpolate_infer as ((([]&?)&?)&?) ; cbn in *.
 
-      + exists M, l, r ; split.
-        1: clear -HM ; solve [crush_incl].
-        easy.
-      + exists (TFun M A), (tLam r), (tApp (tVar 0) l⟨↑⟩).
-        split.
-        1: clear -HM Hat ; solve [crush_incl].
-
-        unfold interpolate_tm in *.
-        prod_splitter.
-        1,3: now eauto 20 with typing.
-        1: solve [crush_incl].
-        1: cbn ; rewrite atoms_ren ; set_solver.
-        cbn.
-        rewrite ST_Beta_Fun, <- erl.
-        apply ereflexivity.
-        rewrite sren_s_flip, sren_t_split.
-        substify.
-        now asimpl.
+      all: refold.
+      2: easy.
+      cbn.
+      rewrite ST_Beta_Fun, <- IH.
+      apply ereflexivity.
+      substify.
+      now asimpl.
 
     - (* case tVar *)
-      intros ? n T Hin ?? s c.
-      destruct (find_side s n) as [[]|] eqn:e.
-      3: exfalso ; now eauto using in_context_find_none.
-
-      + right.
-        apply find_side_some_l in e as (n'&A&[? ->]).
-        eapply in_context_inj in Hin.
-        2:now eapply sren_s_ty.
-        subst.
-        split.
-        1: intros ; rewrite atoms_in ; tea ; set_solver.
-
-        exists TUnit, tStar, (tVar (S n')).
-        split.
-        1: intros ; cbn ; set_solver.
-        unfold interpolate_tm.
-        prod_splitter.
-        1,3: eauto with typing.
-        1-2: solve [crush_incl].
-        cbn.
-        now rewrite sren_t_split.
-
-      + left.
-        apply find_side_some_r in e as (n'&A&[? ->]).
-        eapply in_context_inj in Hin.
-        2:now eapply sren_t_ty.
-        subst.
-        split.
-        1: intros ; rewrite atoms_in ; tea ; set_solver.
-
-        exists TUnit, tStar, (tVar (S n')).
-        split.
-        1: solve [crush_incl].
-
-        unfold interpolate_tm.
-        prod_splitter.
-        1,3: eauto with typing.
-        1-2: solve [crush_incl].
-        reflexivity. 
+      intros * Hin * Hs.
+      destruct (find_side s n) as ([[]|]&?) eqn:e.
+      + eapply find_side_some_l in e as (A&[? ->]) ; tea ; cbn.
+        reflexivity.
+      + eapply find_side_some_r in e as (A&[? ->]) ; tea ; cbn.
+        reflexivity.
+      + exfalso ; now eauto using in_context_find_none.
 
     - (* case tConst *)
-      intros Γ c ?? ? csplit.
-      destruct (const_cover csplit c).
-      
-      + right.
-        split.
-        1: now right ; eexists.
-
-        exists TUnit, tStar, (tConst c).
-        split.
-        1: solve [crush_incl].
-        red ; prod_splitter.
-        1,3: now eauto with typing.
-        1-2: crush_incl.
-
-        reflexivity.
-      
-      + left.
-        split.
-        1: now right ; eexists.
-
-        exists TUnit, tStar, (tConst c).
-        split.
-        1: solve [crush_incl].
-        red ; prod_splitter.
-        1,3: now eauto with typing.
-        1-2: crush_incl.
-
-        reflexivity.
+      intros * Hs.
+      destruct const_cover ; cbn.
+      all: reflexivity.
 
     - (* case tApp *)
-      intros Γ A B n u _ Hn _ IHu Γs Γt s c.
-      destruct (Hn _ _ s c) as
-        [[IHpol (Mt&lt&rt&(IHt&?&?&?&?&et))]|[IHpol (Mt&lt&rt&(IHt&?&?&?&?&et))]].
+      intros * ? IHf _ IHu * Hs.
+      specialize (IHf _ _ _ c Hs).
+      destruct interpolate_infer as ((([]&?)&?)&?) ; cbn in *.
+      all: red ; erewrite infer_infer ; tea ; cbn.
+      
+      + specialize (IHu _ _ _ (flip_csplit c) (flip_splits _ Hs)) ; cbn in *.
+        destruct interpolate as ((?&?)&?) ; cbn.
+        rewrite sren_s_flip, sren_t_split in IHu.
+        now rewrite !tip_up_ren, !tip_subst, ST_Fst, ST_Snd, IHf, IHu.
 
-      + left.
-        cbn in *.
-        specialize (IHu _ _ s c) as (Mu&lu&ru&(IHMu&?&?&?&?&eu)).
-        split.
-        1: clear -IHpol IHt IHMu ; solve [crush_incl].
-        exists (TProd Mt Mu), (tPair lt lu),
-          (tApp (rt[tip tFst]) (ru[(tip tSnd)])).
-        cbn.
-        split.
-        1: clear -IHpol IHt IHMu ; solve [crush_incl].
-
-        unfold interpolate_tm in *.
-        prod_splitter.
-        1,3: now eauto 20 with typing.
-        1: solve [crush_incl].
-        1:{
-          cbn.
-          erewrite union_mono.
-          2,3: rewrite atoms_tm_subst, atoms_subst_tip ; cbn ; reflexivity.
-          set_solver.
-        }
-        cbn.
-        now rewrite !tip_up_ren, !tip_subst, ST_Fst, ST_Snd, eu, et.
-
-      + right.
-        cbn in *.
-        specialize (IHu _ _ (flip_split s) (flip_csplit c)) as (Mu&lu&ru&(IHMu&?&?&?&?&eu)).
-        split.
-        1: clear -IHpol IHt IHMu ; solve [crush_incl].
-        exists (TProd Mt Mu), (tPair lt lu),
-          (tApp (rt[tip tFst]) (ru[tip tSnd])).
-        cbn.
-        split.
-        1: clear -IHpol IHt IHMu; solve [crush_incl].
-        
-        unfold interpolate_tm in *.
-        prod_splitter.
-        1,3: now eauto 20 with typing.
-        1: solve [crush_incl].
-        1:{
-          cbn.
-          erewrite union_mono.
-          2,3: rewrite atoms_tm_subst, atoms_subst_tip ; cbn ; reflexivity.
-          set_solver.
-        }
-        cbn.
-        now rewrite !tip_up_ren, !tip_subst, ST_Fst, ST_Snd, eu, et.
+      + specialize (IHu _ _ _ c Hs) ; cbn in *.
+        destruct interpolate as ((?&?)&?) ; cbn.
+        now rewrite !tip_up_ren, !tip_subst, ST_Fst, ST_Snd, IHf, IHu.
 
     - (* case tProj *)
-      intros * _ IH Γs Γt s c.
-      destruct (IH _ _ s c) as [[IHb (M&l&r&(HM&?&?&?&?&etm))]|[IHb (M&l&r&(HM&?&?&?&?&etm))]].
-      + left.
-        split.
-        1: destruct b ; clear -HM IHb ; solve [crush_incl].
-        exists M, l, (tProj b r).
-        split.
-        1: solve [crush_incl].
+      intros * _ IH * Hs.
+      specialize (IH _ _ _ c Hs).
+      destruct interpolate_infer as ((([]&?)&?)&?) ; cbn in *.
+      all: now rewrite IH.
 
-        unfold interpolate_tm in * ; prod_splitter.
-        3: destruct b.
-        1,3,4: now eauto with typing.
-        1-2: easy.
-        cbn.
-        now rewrite etm.
-      
-      + right.
-        split.
-        1: destruct b ; clear -HM IHb ; solve [crush_incl].
-
-        exists M, l, (tProj b r).
-        split ; [easy|].
-        unfold interpolate_tm in * ; prod_splitter.
-        3: destruct b ; cbn.
-        1,3,4: now eauto with typing.
-        1-2: easy.
-        cbn.
-        now rewrite etm.
   Qed.
 
 End Interpolation.
